$\phi(-1)+\phi(1)=\phi(-1+1)=\phi(0)=0$

$\phi(1/2)\times\phi(2)=\phi(\frac{1}{2}\times2)=\phi(1)=1$

$\phi(\frac{1}{2})=\frac{1}{2}$

$\phi(\frac{6}{7})\times\phi(7)=\phi(\frac{6}{7}\times7)=6$

$\phi(\frac{6}{7})=\frac{6}{7}$

$1+i^2=0$

$\phi(1+i^2)=\phi(0)$

$\phi(1+i^2)=0$

$\phi(1)+\phi(i^2)=0$

$\phi(i^2)=-1$

$\phi(i)=i,-i$

$\phi_\alpha(i)=i$

$\phi_\beta(1)=1$

$\phi_\beta(1+i)=1-i$

$\phi_\alpha(2i)=2i$

$\mathbb{Q}[i]$ then has two homomorphisms

Now talking about $\mathbb{Q}[\zeta]$

$\zeta^2+\zeta+1=0$

$\phi(\zeta^2+\zeta)=-1$

$\phi(\zeta^2)+\phi(\zeta)+1=0$

$\phi(\zeta)^2+\phi(\zeta)+1=0$

Roots are $\zeta,\zeta^2$

$\phi(\zeta)=\zeta,\zeta^2$

$\phi_\alpha(\zeta)=\zeta$

$\phi_\beta(\zeta)=\zeta^2$

$\phi_\beta(a+b\zeta)$

$=\phi_\beta(a)+\phi_\beta(b)\phi_\beta(\zeta)$

$=a+b(-\zeta-1)$

$=a-b-b\zeta$

$\phi_\alpha(a+b\zeta)=a+b\zeta$ which is the identity

$\mathbb{Q}[\sqrt[3]2]$

$\sqrt[3]2=\gamma$

$\gamma$ satisfies $x^3-2=0$

$(\gamma\zeta)^3=2$

$(\gamma\zeta^2)^3=2$

![[Pasted image 20220202205424.png]]

Because we multiply by $\zeta$ which is not inside $\mathbb{Q}[\gamma]$ we know that $\sqrt[3]2$ maps to $\sqrt[3]2$

$\zeta=-\frac{1}{2}+\frac{\sqrt{3}}{2i}$

